#+STARTUP: showall
Propositional Equivalence

* Some definitions
** A proposition that is always true is a *tautology*.
** A proposition that is always false is a *contradiction*
** A proposition that is neither a tautology or a contradiction is a *contingency*
| $p$ | $\lnot p$   | $p \lor \lnot p$ | $p \land \lnot p$ |
| F   | T           | T                | F                 |
| T   | F           | T                | F                 |
|     | contingency | tautology        | contradiction     |

* Logical equivalence
** If proposition $p$ and $q$ have the same truth value for every assignment of truth values to their constituent propositions, the two propositions are *logically equivalent*
** This is written $p \equiv q$
*** Equivalent is typed with \equiv
** $p \equiv q$ is the same as saying $p \leftrightarrow q$ is a tautology

** Example: Show that $\lnot(p \rightarrow q)$ is logically equivalent to the proposition $p \land \lnot q$
|     |     | a                        | b                 |                       |
| $p$ | $q$ | $\lnot(p \rightarrow q)$ | $p \land \lnot q$ | $a \leftrightarrow b$ |
| F   | F   | F                        | F                 | T                     |
| F   | T   | F                        | F                 | T                     |
| T   | F   | T                        | T                 | T                     |
| T   | T   | F                        | F                 | T                     |

* Some propositional equivalences
** Identity
$p \land T \equiv p$
$p \lor F \equiv p$

** Double negation
$\lnot \lnot p \equiv p$

** Domination
$p \lor T \equiv T$
$p \land F \equiv F$

** Idempotent
$p \land p \equiv p$
$p \lor p \equiv p$

** Commutative
$t \land u \equiv u \land t$
$t \lor u \equiv u \lor t$

** Associative
$(t \land u) \land v \equiv t \land (u \land v)$
$(t \lor u) \lor v \equiv t \lor (u \lor v)$

** Distributive
$a \land (b \lor c) \equiv (a \land b) \lor (a \land c)$
$a \lor (b \land c) \equiv (a \lor b) \land (a \lor c)$

** Demorgan's
$\lnot (p \land q) \equiv \lnot p \lor \lnot q$
$\lnot (p \lor q) \equiv \lnot p \land \lnot q$

** Absorbsion
$r \land (r \land q) \equiv r \land q$
$r \lor (r \lor q) \equiv r \lor q$

** Negation
$p \land \lnot p \equiv \mathrm{F}$
$p \lor \lnot p \equiv \mathrm{T}$
