#+STARTUP: showall

Showing Propositional Equivalence

* How to show two propositions are equivalent. Either
1. Make a truth table for the two propositions.
   - If the two propositions have the same truth value for every assignment of truth values to their variables
   - Or, if the biconditional of the two propositions under consideration is a tautology
   - Then the two propositions are equivalent.
2. Rewrite one of the propositions by applying known propositional equivalences, transforming it, perhaps across multiple steps, into the other proposition under consideration.


* Show that $\lnot (p \rightarrow q)$ and $p \land \lnot q$ are equivalent.
** Truth Table
| $p$ | $q$ | $(p \rightarrow q)$ | $\lnot (p \rightarrow q)$ |
| F   | F   | T                   | F                         |
| F   | T   | T                   | F                         |
| T   | F   | F                   | T                         |
| T   | T   | T                   | F                         |

| $p \land \lnot q$ | $\lnot (p \rightarrow q) \leftrightarrow p \land \lnot q$ |
| F                 | T                                                         |
| F                 | T                                                         |
| T                 | T                                                         |
| F                 | T                                                         |

** Rewriting with well-known equivalences
 Proposition                              Rewritten to                  | Reason
 $\lnot (p \rightarrow q)$      $\equiv$  $\lnot (\lnot p \lor q)$      | Table 7 (book)
 $\lnot (\lnot p \lor q)$       $\equiv$  $\lnot \lnot p \land \lnot q$ | DeMorgan's
 $\lnot \lnot p \land \lnot q$  $\equiv$  $p \land \lnot q$             | Double Negative

* Show DeMorgan's Law for negated and.

** To be shown: $\lnot (p \land q) \equiv \lnot p \lor \lnot q$
** Truth Table
| $p$ | $q$ | $(p \land q)$ | $\lnot (p \land q)$ | $\lnot p \lor \lnot q$ |
| F   | F   | F             | T                   | T                      |
| F   | T   | F             | T                   | T                      |
| T   | F   | F             | T                   | T                      |
| T   | T   | T             | F                   | F                      |
$\therefore$ $\lnot (p \land q) \equiv \lnot p \lor \lnot q$
